\section{Main Results}
We can recurse backwards in \eqref{errprelim} to obtain the following:
\begin{align}\label{errrec}
e_t=F_{t,1}e_0+\ous{\sum}{k=1}{t}\alpha F_{t,k+1}\zeta_k
\end{align}
Looking at \eqref{errrec} it is clear that quantities $F_{t,j}, j=1,\ldots,t$ influence the dyanmics of $e_t$.
\subsection{Additive Noise}
\FloatBarrier
\comment{
\begin{table}
\resizebox{.5\textwidth}{!}{
\begin{tabular}{|l|c|c|}\hline
\theadfont\diagbox[width=3em]{$H$}{$\zeta$}&
\thead{US}&\thead{S}\\    \hline
AS& $\Big(\frac{\norm{\theta_0-\ts}^2_2}{\alpha^2(t+1)^2}+\frac{\sigma^2}{t+1}\Big)\big(1+2nB_1+n^2B_2\big)$  & NA \\    \hline
PS& $\Big(\frac{\norm{\theta_0-\ts}^2_2}{\alpha^2(t+1)^2}+\frac{\sigma^2}{t+1}\Big)\big(1+\frac{2}{1-\norm{F_D}_{op}}+\frac{1}{1-\norm{F_D}^2_{op}}\big)$ &NA\\ \hline
PD& $\Big(\frac{\norm{\theta_0-\ts}^2_2}{\alpha^2(t+1)^2}+\frac{\sigma^2}{t+1}\Big)$
\end{tabular}
}
\end{table}
}
\comment{
\begin{table}
%\resizebox{.5\textwidth}{!}{

\begin{tabular}{|l|c|}\hline
\theadfont\diagbox[width=3em]{$H$}{$\zeta$}&
\thead{Strucutred}\\    \hline
AS& NA  \\    \hline
PS& NA\\ \hline
PD& $\Big(\frac{\norm{\theta_0-\ts}^2_2}{\alpha^2(t+1)^2}+\frac{\sigma^2}{t+1}\Big)$\\\hline
PD& $\Big(\frac{\norm{\theta_0-\ts}^2_2}{\alpha^2(t+1)^2}+\frac{\sigma^2}{t+1}\Big)$\\\hline
\end{tabular}
%}
\end{table}
}
\comment{In the case of additive noise (AN), we have $F_{i,j}= (I-\alpha H)^{i-j+1},~\forall i\geq j$ to be deterministic. In what follows we resort to abuse of notation by letting $F_D=F_{0,0}=I-\alpha H$. The convergence of \eqref{lsa} in the AN case then depends on the spectral properties of $F$, which in turn depends on the choice of $\alpha$ for a given $H$. We are interested in the following two quantities
\begin{enumerate}
\item The \emph{spectral radius} $\rho_s(F_D)$, where $\rho(A)\eqdef\max\{|\lambda_1|,\ldots,|\lambda_k|,k\leq n\}$ with $|\lambda_i|$ denoting the absolute value of the Eigen value $\lambda_i$ of any given matrix $A$.
\item The \emph{operator norm} of $\norm{F_D}_{op}$, where $\norm{A}_{op}\eqdef\us{\sup}{x^\top x\leq 1}\sqrt{x^\top A^\top A x}$ is the operator norm of any given matrix $A$.
\end{enumerate}
}
\begin{lemma}\label{addstep}
\begin{enumerate}[label=(\roman*)]
\item For any $H$ that is AS there exists an $\alpha_{as}>0$ for which it holds that $\rho(F_D(\alpha))<1,~\forall \alpha\in (0,\alpha_{as})$.
\item For any $H$ that is PS there exists an $\alpha_{ps}>0$ for which it holds that $\E[x^\top(H-\alpha H_t^\top H_t)x|\F_{t-1}]> 0$, $~\forall \alpha\in (0,\alpha_{ps})$.
\end{enumerate}
\end{lemma}
We begin by stating a result related to norms of matrices
\begin{lemma}
Let $A\in \R^{n\times n}$ be any real matrix then $\norm{Ax}^2_2\leq \us{\sup}{i,j}n^2|(A)_{ij}|^2\norm{x}^2_2$ and $\ip{x,Ax}\leq \us{\sup}{i,j}n|(A)_{ij}|\norm{x}^2_2$, where $(A)_{ij}$ denotes the $ij^{th}$ entry of matrix $A$.
\end{lemma}
\begin{lemma}
For $\alpha \in (0,\alpha_{as})$ there exists constants $B_1>0$ and $B_2>0$ such that $B_1=\us{\us{\sup}{i,j}}{t\geq 0}|(F_D^t)_{ij}|$ and $B_2=\us{\us{\sup}{i,j}}{t\geq 0}|(F_D^{t\top}F_D^t)_{ij}|$
\end{lemma}
\begin{align}
\eb_t&=\frac{1}{t+1}(\ous{\sum}{i=0}{t} F_{i,1} e_0+ \alpha\ous{\sum}{i=1}{t} \ous{\sum}{k=i}{t} F_{k,i+1}  \zeta_i )\nn\\
&=\frac{1}{t+1}\big((\alpha H)^{-1}(I-F_D^t)e_0+ H^{-1}\ous{\sum}{i=1}{t}(I-F_D^{t-i}) \zeta_i\big)
\end{align}
\begin{table*}
\begin{center}
\resizebox{1\textwidth}{!}{
\begin{tabular}{|c|c|c|c|c|}\hline
Matrix   & $\alpha$             &   $C$     & Noise     &   $E[\norm{C\eb_t}^2]\leq \B^2+\V^2$\\\hline
AS       & $(0,\alpha_{as})$    &   $H$     & AUS        &   $\B^2=\Big(\frac{\norm{\theta_0-\ts}^2_2}{\alpha^2(t+1)^2}\Big)\big(1+2nB_1+n^2B_2\big),~\V^2=\Big(\frac{\sigma^2}{t+1}\Big)\big(1+2nB_1+n^2B_2\big)$\\    \hline
AS       & $(0,\alpha_{as})$    &   $I$     & AUS        &   $\B^2=\norm{H^{-1}}^2\Big(\frac{\norm{\theta_0-\ts}^2_2}{\alpha^2(t+1)^2}\Big)\big(1+2nB_1+n^2B_2\big),~\V^2=\norm{H^{-1}}^2\Big(\frac{\sigma^2}{t+1}\Big)\big(1+2nB_1+n^2B_2\big)$\\    \hline

PS       & $(0,\alpha_{ps})$    &   $H$     & AUS        &   $\B^2=\Big(\frac{\norm{\theta_0-\ts}^2_2}{\alpha^2(t+1)^2}\Big)\big(1+2(1-\alpha\frac{\rho_H}{2})^t+(1-\alpha\rho_H)^t\big),~\V^2=\Big(\frac{\sigma^2}{t+1}\Big)\big(1+5\alpha^{-1}{\rho_H}^{-1})$\\ \hline
PS       & $(0,\alpha_{ps})$    &   $I$     & AUS        &   $\B^2=\norm{H^{-1}}^2\Big(\frac{\norm{\theta_0-\ts}^2_2}{\alpha^2(t+1)^2}\Big)\big(1+2(1-\alpha\frac{\rho_H}{2})^t+(1-\alpha\rho_H)^t\big),~\V^2=\norm{H^{-1}}^2\Big(\frac{\sigma^2}{t+1}\Big)\big(1+5\alpha^{-1}{\rho_H}^{-1})$\\ \hline

SPDS    & $(0,\alpha_{ps})$     &   $H$     & AUS        &   $\B^2=\frac{\norm{\theta_0-\ts}^2_2}{\alpha^2(t+1)^2},~\V^2=\frac{\sigma^2}{t+1}$\\ \hline
SPDS    & $(0,\alpha_{ps})$     &   $H^{\frac{1}{2}}$     & US        &   $\B^2=\norm{H^{-1}}\frac{\norm{\theta_0-\ts}^2_2}{\alpha^2(t+1)^2},~\V^2=\norm{H^{-1}}\frac{\sigma^2}{t+1}$\\ \hline
SPDS    & $(0,\alpha_{ps})$     &   $H^{\frac{1}{2}}$     & US        &   $\B^2=\norm{H^{-1}}\frac{\norm{\theta_0-\ts}^2_2}{\alpha^2(t+1)^2},~\V^2=\norm{H^{-1}}\frac{\sigma^2}{t+1}$\\ \hline

SPDS    & $(0,\alpha_{ps})$     &   $I$     & AUS        &   $\B^2=\norm{H^{-1}}^2\frac{\norm{\theta_0-\ts}^2_2}{\alpha^2(t+1)^2},~\V^2=\norm{H^{-1}}^2\frac{\sigma^2}{t+1}$\\ \hline
SPDS    & $(0,\alpha_{ps})$     &   $I$     & AS        &   $\B^2=\norm{H^{-1}}^2\frac{\norm{\theta_0-\ts}^2_2}{\alpha^2(t+1)^2},~\V^2=\norm{H^{-1}}\frac{\sigma^2}{t+1}$\\ \hline
SPDS    & $(0,\alpha_{ps})$     &   $H^{\frac{1}{2}}$     &AS        &   $\B^2=\frac{\norm{H^{-\frac{1}{2}}(\theta_0-\ts)}^2_2}{\alpha^2(t+1)^2},~\V^2=\frac{\sigma^2}{t+1}$\\ \hline
PS       & $(0,\alpha_{ps})$    &   $I$     & MUS        &   $\B^2=\frac{(\rho_H\alpha)^{-1}(1+4(\rho_H\alpha)^{-1})}{(t+1)^2},~\V^2=(\sigma^2)\frac{\alpha^2(\alpha\rho_H)^{-1}(1+4(\rho_H\alpha)^{-1})}{t+1}$\\ \hline
SPDS    & $(0,\alpha_{ps})$     &   $H$     & MUS        &  $\B^2=\frac{\norm{\theta_0-\ts}^2_2}{\alpha^2(t+1)^2},~\V^2=\frac{\sigma^2}{t+1}$\\ \hline
SPDS    & $(0,\alpha_{ps})$     &   $H^{\frac{1}{2}}$     & MUS        &   $\B^2=\frac{(\rho_H)^{-1}(\alpha)^{-2}}{(t+1)^2},~\V^2=(\sigma^2)\frac{(\rho_H)^{-1}}{t+1}$\\ \hline
SPDS    & $(0,\alpha_{ps})$     &   $H^{\frac{1}{2}}$     & MS        &   $\B^2=\frac{\norm{H^{-\frac{1}{2}}(\theta_0-\ts)}^2_2}{\alpha^2(t+1)^2},~\V^2=\frac{\sigma^2}{t+1}$\\ \hline
\end{tabular}
}
\end{center}
\end{table*}
\begin{theorem}
In the case of additive noise, i.e., $M_t=0$, \\
\textbf{Unstructured Noise}
\begin{enumerate}[label=(\roman*)]
\item if $H$ is AS, then $\forall \alpha\in (0,\alpha_{as})$ and $t\geq0 $ we have $E\norm{H\eb_t}^2\leq \Big(\frac{\norm{\theta_0-\ts}^2_2}{\alpha^2(t+1)^2}+\frac{\sigma^2}{t+1}\Big)\big(1+2nB_1+n^2B_2\big)$.
\item if $H$ is PS, then $\forall \alpha \in (0,\alpha_{ps})$ and $t\geq 0$ we have $E\norm{H\eb_t}^2\leq \Big(\frac{\norm{\theta_0-\ts}^2_2}{\alpha^2(t+1)^2}+\frac{\sigma^2}{t+1}\Big)\big(1+\frac{2}{1-\norm{F_D}_{op}}+\frac{1}{1-\norm{F_D}^2_{op}}\big)$.
\item if $H$ is PD, then $\forall \alpha \in (0,\alpha_{ps})$ and $t\geq 0$ we have $E\norm{H\eb_t}^2\leq \Big(\frac{\norm{\theta_0-\ts}^2_2}{\alpha^2(t+1)^2}+\frac{\sigma^2}{t+1}\Big)$.
\item if $H$ is PD, then $\forall \alpha \in (0,\alpha_{ps})$ and $t\geq 0$ we have $E\norm{H^{\frac{1}{2}}\eb_t}^2\leq \norm{H^{-1}}^2_{op}\Big(\frac{\norm{(\theta_0-\ts)}^2_2}{\alpha^2(t+1)^2}+\frac{\sigma^2}{t+1}\Big)$.
\end{enumerate}
\textbf{Structured Noise}
\begin{enumerate}[label=(\roman*)]
\item if $H$ is PD, then $\forall \alpha \in (0,\alpha_{ps})$ and $t\geq 0$ we have $E\norm{H^{\frac{1}{2}}\eb_t}^2\leq \Big(\frac{\norm{H^{-\frac{1}{2}}(\theta_0-\ts)}^2_2}{\alpha^2(t+1)^2}+\frac{\sigma^2}{t+1}\Big)$
\end{enumerate}
\end{theorem}


\begin{theorem}
In the case of additive noise, i.e., $M_t=0$, \\
\textbf{Unstructured Noise}
\begin{enumerate}[label=(\roman*)]
\item if $H$ is AS, then $\forall \alpha\in (0,\alpha_{as})$ and $t\geq0 $ we have $E\norm{\eb_t}^2\leq \Big(\frac{\norm{\theta_0-\ts}^2_2}{\alpha^2(t+1)^2}+\frac{\sigma^2}{t+1}\Big)\big(1+2nB_1+n^2B_2\big)$.
\item if $H$ is PS, then $\forall \alpha \in (0,\alpha_{ps})$ and $t\geq 0$ we have $E\norm{\eb_t}^2\leq \Big(\frac{\norm{\theta_0-\ts}^2_2}{\alpha^2(t+1)^2}+\frac{\sigma^2}{t+1}\Big)\big(1+\frac{2}{1-\norm{F_D}_{op}}+\frac{1}{1-\norm{F_D}^2_{op}}\big)$.
\item if $H$ is PD, then $\forall \alpha \in (0,\alpha_{ps})$ and $t\geq 0$ we have $E\norm{\eb_t}^2\leq \Big(\frac{\norm{\theta_0-\ts}^2_2}{\alpha^2(t+1)^2}+\frac{\sigma^2}{t+1}\Big)$.
\end{enumerate}
\textbf{Structured Noise}
\begin{enumerate}[label=(\roman*)]
\item if $H$ is PD, then $\forall \alpha \in (0,\alpha_{ps})$ and $t\geq 0$ we have $E\norm{\eb_t}^2\leq \Big(\frac{\norm{H^{-\frac{1}{2}}(\theta_0-\ts)}^2_2}{\alpha^2(t+1)^2}+\frac{\sigma^2}{t+1}\Big)$
\end{enumerate}
\end{theorem}

\comment{
\begin{theorem}[AS-AN]
When $H$ is AS and $M_t=0,\forall t\geq 0$, we have
\begin{align}
E\norm{H\eb_t}\leq \Big(\frac{\norm{\theta_0-\ts}^2_2}{\alpha^2(t+1)^2}+\frac{\sigma^2}{t+1}\Big)\big(1+2nB_1+n^2B_2\big)
\end{align}
\end{theorem}
\begin{theorem}[PS-AN]
When $H$ is PS, $M_t=0,\forall t\geq 0$ and $\alpha\in (0,\alpha_{ps})$
\begin{align}
E\norm{H\eb_t}\leq \Big(\frac{\norm{\theta_0-\ts}^2_2}{\alpha^2(t+1)^2}+\frac{\sigma^2}{t+1}\Big)\big(1+\frac{2}{1-\norm{F_D}_{op}}+\frac{1}{1-\norm{F_D}^2_{op}}\big)
\end{align}
\end{theorem}
\begin{theorem}[SPDS-AN]
When $H$ is SPDS and $M_t=0,\forall t\geq 0$, and $\alpha\in (0,\alpha_{ps})$
\begin{align}
E\norm{H\eb_t}\leq \Big(\frac{\norm{\theta_0-\ts}^2_2}{\alpha^2(t+1)^2}+\frac{\sigma^2}{t+1}\Big)
\end{align}
\end{theorem}
\begin{theorem}[SPDS-Structured Noise]
When $H$ is SPDS and $M_t=0,\forall t\geq 0$, and $\alpha\in (0,\alpha_{ps})$
\begin{align}
E\norm{H^{\frac{1}{2}}\eb_t}\leq \Big(\frac{\norm{H^{-\frac{1}{2}}(\theta_0-\ts)}^2_2}{\alpha^2(t+1)^2}+\frac{\sigma^2}{t+1}\Big)
\end{align}
\end{theorem}
\begin{theorem}[SPDS-Unstructured Noise]
When $H$ is SPDS and $M_t=0,\forall t\geq 0$, and $\alpha\in (0,\alpha_{ps})$
\begin{align}
E\norm{H^{\frac{1}{2}}\eb_t}\leq \norm{H^{-1}}^2_{op}\Big(\frac{\norm{(\theta_0-\ts)}^2_2}{\alpha^2(t+1)^2}+\frac{\sigma^2}{t+1}\Big)
\end{align}
\end{theorem}
}
