<<<<<<< Updated upstream
%!TEX root =  lsa.tex
\section{Proof}
\label{sec:proof}
%%%%%%%%%%%%%%%%%%%%%%%%%%%%%%%%%%%%%%%%
In this section we provide the proof of \cref{maintheorem}.
=======
\section{Proof of \Cref{maintheorem}}
\begin{proof}
$\E[\norm{H\eb_t}^2]=\E\ip{H\eb_t,H\eb_t}=\frac{1}{(t+1)^2}\E\ip{H\ous{\sum}{i=0}{t}(\theta_i-\ts),H\ous{\sum}{i=0}{t}(\theta_i-\ts)}$.
$\E\ous{\sum}{i=0}{t}\ous{\sum}{j=0}{t}\ip{H(\theta_i-\theta^*),H(\theta_j-\theta^*)}=\E\ous{\sum}{i=0}{t}\ip{H(\theta_i-\theta^*),H(\theta_j-\theta^*)}+ 2\E\ous{\sum}{i=0}{t-1}\ous{\sum}{j=i+1}{t}\ip{H(\theta_i-\theta^*),H(\theta_j-\theta^*)}$. Now
\begin{align}\label{inter}
&\E\ous{\sum}{i=0}{t-1}\ous{\sum}{j=i+1}{t}\ip{H(\theta_i-\theta^*),H(\theta_j-\theta^*)}\nn\\
&=\E\ous{\sum}{i=0}{t-1}\ous{\sum}{j=i+1}{t}\ip{H(\theta_i-\theta^*),H\big[F_{j,i+1} (\theta_i-\theta^*)+\alpha\sum_{k=i+1}^j F_{j,k+1}\zeta_{k}\big]}\nn\\
&=\E\ous{\sum}{i=0}{t-1}\ous{\sum}{j=i+1}{t}\ip{H(\theta_i-\theta^*),H F_{j,i+1} (\theta_i-\theta^*)}\nn\\
&=\E\ous{\sum}{i=0}{t-1}\ous{\sum}{j=i+1}{t}\ip{H(\theta_i-\theta^*),H(I-\alpha H)^{j-i} (\theta_i-\theta^*)}\nn\\
&=2(\alpha\rho_{\alpha})^{-1}\E\ous{\sum}{i=0}{t-1}\ip{H(\theta_i-\theta^*),H (\theta_i-\theta^*)}\nn\\
&\leq2(\alpha\rho_{\alpha})^{-1}\E\ous{\sum}{i=0}{t}\ip{H(\theta_i-\theta^*),H (\theta_i-\theta^*)}\nn\\
\end{align}
$\E\ous{\sum}{i=0}{t}\ous{\sum}{j=0}{t}\ip{H(\theta_i-\theta^*),H(\theta_j-\theta^*)}=\E\ous{\sum}{i=0}{t}(1+4(\alpha\rho_{\alpha})^{-1})\ip{H(\theta_i-\theta^*),H(\theta_i-\theta^*)}$

Now
\begin{align*}
\E\ip{H(\theta_i-\theta^*),H(\theta_i-\theta^*)}=\E\ip{F_{i,1}e_0,F_{i,1}e_0}+\ous{\sum}{j=1}{i}\E\ip{F_{i,j+1}\zeta_j,F_{i,j+1}\zeta_j}
\leq (1-\alpha\rho_{\alpha})^i+ (\alpha\rho_{\alpha})^{-1}\sigma^2
\end{align*}
$\E\ous{\sum}{i=0}{t}\ous{\sum}{j=0}{t}\ip{H(\theta_i-\theta^*),H(\theta_j-\theta^*)}\leq (1+4(\alpha\rho_{\alpha})^{-1}) (\alpha\rho_{\alpha})^{-1}(t\sigma^2+\norm{\theta_0-\ts}^2)$
\begin{align}
\E[\norm{H\eb_t}]\leq (1+4(\alpha\rho_{\alpha})^{-1}) (\alpha\rho_{\alpha})^{-1} \Big(\frac{\norm{\theta_0-\ts}^2}{(t+1)^2}+ \frac{\alpha^2\sigma^2}{t+1} \Big)
\end{align}
\end{proof}

>>>>>>> Stashed changes
