\begin{table*}[t]
\begin{center}
\resizebox{1\textwidth}{!}{
\begin{tabular}{|c|c|c|c|c|c|c|}\hline
Matrix   & $\alpha$             &   $C$     & Noise     &   $\B^2$ &\V^2$   & Work \\\hline
AS       & $(0,\alpha_{as})$    &   $H$     & AN        &   $\B^2=\Big(\frac{\norm{e_0}^2_2}{\alpha^2(t+1)^2}\Big)\big(1+2nB_1+n^2B_2\big)$& $\V^2=\Big(\frac{\sigma^2}{t+1}\Big)\big(1+2nB_1+n^2B_2\big)$& New \\   \hline

PS       & $(0,\alpha_{ps})$    &   $H$     & AN        &   $\B^2=\Big(\frac{\norm{e_0}^2_2}{\alpha^2(t+1)^2}\Big)\big(1+2(1-\alpha\frac{\rho_H}{2})^t+(1-\alpha\rho_H)^t\big)$& $\V^2=\Big(\frac{\sigma^2}{t+1}\Big)\big(1+5\alpha^{-1}{\rho_H}^{-1})$& New \\   \hline

SPDS    & $(0,\alpha_{ps})$     &   $H$     & AN        &   $\B^2=\frac{\norm{e_0}^2_2}{\alpha^2(t+1)^2}$& $\V^2=\frac{\sigma^2}{t+1}$& New \\   \hline

SPDS    & $(0,\alpha_{ps})$     &   $H^{\frac{1}{2}}$     & AN        &   $\B^2=\norm{H^{-1}}\frac{\norm{e_0}^2_2}{\alpha^2(t+1)^2}$& $\V^2=\norm{H^{-1}}\frac{\sigma^2}{t+1}$& New \\   \hline
SPDS    & $(0,\alpha_{ps})$     &   $H^{\frac{1}{2}}$     &AN+SN        &   $\B^2=\frac{\norm{H^{-\frac{1}{2}}(e_0)}^2_2}{\alpha^2(t+1)^2}$& $\V^2=\frac{\sigma^2}{t+1}$& \cite{} \\   \hline

AS       & $(0,\alpha_{as})$    &   $I$     & AN        &   $\B^2=\norm{H^{-1}}^2\Big(\frac{\norm{e_0}^2_2}{\alpha^2(t+1)^2}\Big)\big(1+2nB_1+n^2B_2\big)$& $\V^2=\norm{H^{-1}}^2\Big(\frac{\sigma^2}{t+1}\Big)\big(1+2nB_1+n^2B_2\big)$& New \\   \hline
PS       & $(0,\alpha_{ps})$    &   $I$     & AN        &   $\B^2=\norm{H^{-1}}^2\Big(\frac{\norm{e_0}^2_2}{\alpha^2(t+1)^2}\Big)\big(1+2(1-\alpha\frac{\rho_H}{2})^t+(1-\alpha\rho_H)^t\big)$& $\V^2=\norm{H^{-1}}^2\Big(\frac{\sigma^2}{t+1}\Big)\big(1+5\alpha^{-1}{\rho_H}^{-1})$& New \\   \hline

SPDS    & $(0,\alpha_{ps})$     &   $I$     & AN        &   $\B^2=\norm{H^{-1}}^2\frac{\norm{e_0}^2_2}{\alpha^2(t+1)^2}$& $\V^2=\norm{H^{-1}}^2\frac{\sigma^2}{t+1}$& New \\   \hline
SPDS    & $(0,\alpha_{ps})$     &   $I$     & AN+SN        &   $\B^2=\norm{H^{-1}}^2\frac{\norm{e_0}^2_2}{\alpha^2(t+1)^2}$& $\V^2=\norm{H^{-1}}\frac{\sigma^2}{t+1}$& New \\   \hline
SPDS    & $(0,\alpha_{ps})$     &   $H$     & MN        &  $\B^2=\frac{\norm{e_0}^2_2}{\alpha^2(t+1)^2}$& $\V^2=\frac{\sigma^2}{t+1}$& New \\   \hline
SPDS    & $(0,\alpha_{ps})$     &   $H^{\frac{1}{2}}$     & MN        &   $\B^2=\frac{\norm{H^{-1}}}{\alpha^2(t+1)^2}$& $\V^2=(\sigma^2)\frac{\norm{H^{-1}}}{t+1}$& New \\   \hline
PS       & $(0,\alpha_{ps})$    &   $I$     & MN        &   $\B^2=(1+4(\alpha\rho_H)^{-1}) (\alpha\rho_H)^{-1} \Big(\frac{\norm{e_0}^2}{(t+1)^2}\Big)$& $\V^2=(1+4(\alpha\rho_H)^{-1}) (\alpha\rho_H)^{-1} \Big(\frac{\alpha^2\sigma^2}{t+1} \Big)$& New \\   \hline
SPDS    & $(0,\alpha_{ps})$     &   $H^{\frac{1}{2}}$     & MN_+SN        &   $\B^2=\frac{\norm{H^{-\frac{1}{2}}(e_0)}^2_2}{\alpha^2(t+1)^2}$& $\V^2=\frac{\sigma^2}{t+1}$& \cite{} \\   \hline
\end{tabular}
}
\end{center}
\caption{Main Result}
\label{maintable}
\end{table*}
