\onecolumn
\section{Supplementary Material}
In the case of additive noise, since $M_t=0$, we have $F_{i,j}=F^{i-j}_D$ and hence
\begin{align}\label{addexp}
\eb_t&=\frac{1}{t+1}(\ous{\sum}{i=0}{t} F_{i,1} e_0+ \alpha\ous{\sum}{i=1}{t} \ous{\sum}{k=i}{t} F_{k,i+1}  \zeta_i )
\end{align}
\begin{theorem}
When $H$ is AS, $\alpha \in (0,\alpha_{as})$, we have
$\E[\norm{H\eb_t}^2]\leq \Big(\frac{\norm{\theta_0-\ts}^2_2}{\alpha^2(t+1)^2}\Big)\big(1+2nB_1+n^2B_2\big)+\Big(\frac{\sigma^2}{t+1}\Big)\big(1+2nB_1+n^2B_2\big)$
\end{theorem}
\begin{proof}
Since $\alpha\in (0,\alpha_{as})$, we have from \eqref{addexp}
\begin{align*}
H\eb_t&=H\Big(\frac{1}{t+1}(\ous{\sum}{i=0}{t} F_{i,1} e_0+ \alpha\ous{\sum}{i=1}{t} \ous{\sum}{k=i}{t} F_{k,i+1}  \zeta_i )\Big)\\
&=H\Big(\frac{1}{t+1}\big((\alpha H)^{-1}(I-(I-\alpha H)^t)e_0+ H^{-1}\ous{\sum}{i=1}{t}(I-(I-\alpha H)^{t-i}) \zeta_i\big)\Big)\\
&=\frac{1}{t+1}\big((\alpha)^{-1}(I-(I-\alpha H)^t)e_0+ \ous{\sum}{i=1}{t}(I-(I-\alpha H)^{t-i}) \zeta_i\big)
\end{align*}
Now
\begin{align*}
&\E[\norm{H\eb_t}^2]\\
&=\E\ip{H\eb_t,H\eb_t}\\
&=\frac{1}{\alpha^2(t+1)^2}\E\ip{(I-(I-\alpha H)^t)e_0,(I-(I-\alpha H)^t)e_0}+\frac{1}{(t+1)^2}\ous{\sum}{i=1}{t}\E\ip{(I-(I-\alpha H)^{t-i}) \zeta_i,(I-(I-\alpha H)^{t-i}) \zeta_i}
\end{align*}
Note that for $x\in \R^n$, $\ip{(I-(I-\alpha H)^t)x,(I-(I-\alpha H)^t)x}\leq \ip{x,x}+2\ip{x,(I-\alpha H)^tx}+\ip{(I-\alpha H)^t,(I-\alpha H)^t x}$. Thus it follows that
\begin{align*}
&\E[\norm{H\eb_t}^2]\leq \frac{\norm{\theta_0-\ts}^2}{(t+1)^2} (1+2nB_1+n^2B_2)+\ous{\sum}{i=1}{t}\frac{\sigma^2}{(t+1)^2}(1+2nB_1+n^2B_2)
\end{align*}
\end{proof}


\begin{theorem}
When $H$ is PS, $\alpha \in (0,\alpha_{ps})$, we have
$\E[\norm{H\eb_t}^2]\leq \Big(\frac{\norm{\theta_0-\ts}^2_2}{\alpha^2(t+1)^2}\Big)\big(1+2(1-\alpha\frac{\rho_H}{2})^t+(1-\alpha\rho_H)^t\big)+\Big(\frac{\sigma^2}{t+1}\Big)\big(1+5\alpha^{-1}{\rho_H}^{-1}\big)$
\end{theorem}
\begin{proof}
Note that $\ip{x,(I-\alpha H)^t,x}\leq (1-\alpha\frac{\rho_H}{2})^t \ip{x,x}$, $\ous{\sum}{i=1}{t} 2 (1-\alpha \frac{\rho_H}{2})^{t-i}+(1-\alpha {\rho_H})^{t-i}\leq \ous{\sum}{i=1}{\infty} 2 (1-\alpha \frac{\rho_H}{2})^{t-i}+(1-\alpha {\rho_H})^{t-i}=5\alpha^{-1}\rho_H^{-1}$
\end{proof}

\begin{theorem}
When $H$ is SDPS, $\alpha \in (0,\alpha_{ps})$, we have
$\E[\norm{H\eb_t}^2]\leq \frac{\norm{\theta_0-\ts}^2_2}{\alpha^2(t+1)^2}+\frac{\sigma^2}{t+1}$
\end{theorem}
\begin{proof}
Note that for $x\in \R^n$, $\ip{(I-(I-\alpha H)^t)x,(I-(I-\alpha H)^t)x}\leq \ip{x,x}$
\end{proof}

\begin{theorem}
When $H$ is SDPS and the noise is structured, $\alpha \in (0,\alpha_{ps})$, we have
$\E[\norm{H^{\frac{1}{2}}\eb_t}^2]\leq \frac{\norm{\theta_0-\ts}^2_2}{\alpha^2(t+1)^2}+\frac{\sigma^2}{t+1}$
\end{theorem}
\begin{proof}
\begin{align*}
&\E[\norm{H^{\frac{1}{2}}\eb_t}^2]\\
&=\frac{1}{\alpha^2(t+1)^2}\E\ip{H^{-\frac{1}{2}}(I-(I-\alpha H)^t)e_0,H^{-\frac{1}{2}}(I-(I-\alpha H)^t)e_0}+\frac{1}{(t+1)^2}\ous{\sum}{i=1}{t}\E\ip{H^{-\frac{1}{2}}(I-(I-\alpha H)^{t-i}) \zeta_i,H^{-\frac{1}{2}}(I-(I-\alpha H)^{t-i}) \zeta_i}
\end{align*}
Now
\begin{align*}
E\ip{H^{-\frac{1}{2}}(I-(I-\alpha H)^{t-i}) \zeta_i,H^{-\frac{1}{2}}(I-(I-\alpha H)^{t-i}) \zeta_i}&\leq \E\ip{H^{-\frac{1}{2}}\zeta_i,H^{-\frac{1}{2}}\zeta_i}\\
&=\E trace(H^{-1}\zeta_i\zeta_i^\top)\\
&\leq \sigma^2
\end{align*}

\end{proof}


\begin{lemma}
For any $x_{i-1}\in \R^n$ that is $\F_{i-1}$ measurable and $\forall ~t > i$ if follows that $\E[x_i^\top F_{t,i+1}\zeta_{i}]=0$
\end{lemma}
\small
\begin{proof}
\begin{align*}
&\E[x_t^\top F_{i,t+1}\zeta_{i}]\\
%=\E\big[\E[ x_{i-1}^\top F_{i,t+1}\zeta_{i}|\F_t]\big]\\
=&\E\Bigg[\E\bigg[\E\Big[\E\big[ x_{i-1}^\top F_{t,i+1}\zeta_{i}|\F_{t}\big]|\F_{t-1}\Big]\ldots|\F_{i-1}\bigg]\Bigg]\\
=&\E\Bigg[ x_{i-1}^\top \E\bigg[\E\Big[\E\big[(I-\alpha H_t)|\F_{t}\big]|\ldots \F_{i}\Big]\zeta_{i}|\F_{i-1}\bigg]\Bigg]\\
=&\E\Bigg[ x_{i-1}^\top \E[(I-\alpha H)^{t-i+1}\zeta_{i}|\F_{i-1}]\Bigg]\\
=&\E\Bigg[ x_{i-1}^\top (I-\alpha H)^{t-i}\E\bigg[\zeta_{i}|\F_{i-1}\bigg]\Bigg]\\
=&0
\end{align*}
\end{proof}

\begin{lemma}
For $i\neq j$, $\E[\ip{F_{t,i+1}\zeta_{i},F_{t,j+1} \zeta_{j}}]=0$
\end{lemma}
\begin{proof}
W.l.o.g  $i>j$
\begin{align}
&\E[\ip{F_{t,i+1} \zeta_{i},F_{t,j+1} \zeta_{j}}]\nn\\
\label{diffindexinter}=&\E\big[\E[ \zeta^\top_{i}(I-\alpha H_{i+1})^\top\ldots(I-\alpha H_t)^\top(I-\alpha H_t)\ldots(I-\alpha H_{j+1}) \zeta_{j}|\F_{t-1}]\big]\\
=&\E\big[ \zeta^\top_{i}(I-\alpha H_{i+1})^\top\ldots\E[(I-\alpha H_t)^\top(I-\alpha H_t)|\F_{t-1}]\ldots(I-\alpha H_{j+1}) \zeta_{j}\big]\\
=&\E\big[ \zeta^\top_{i}(I-\alpha H_{i+1})^\top\ldots C\ldots(I-\alpha H_{j+1}) \zeta_{j}\big]\\
\label{diffindex}=&\E[ \sum_{l} G_l],
\end{align}
where $l$ is any index and $G_l$s in \eqref{diffindex} are terms obtained by expanding the product in \eqref{diffindexinter} using the fact that $H_t=H+M_{t},~\forall t\geq 0$. Note that $G_l$ is a product involving powers of $\alpha H$, matrices such as $M^\top_{q+1}$ and $M_{p+1}$ for some $ i\leq p<t, j\leq q < t$ and vectors $\zeta^\top_i$ and $\zeta^\top_j$.
For any given $G_l$ and let $r(l)$ be the largest index such that either $M^\top_{r(l)+1}$ or $M_{r(l)+1}$ or $\zeta_{r(l)+1}$is present in that term.
\begin{align*}
\E[ \sum_{l} G_l]=  \sum_{l} \E\big[\E[G_l|\F_{r(l)}]\big]=0
\end{align*}
\end{proof}
$\E\ous{\sum}{i=0}{t}\ous{\sum}{j=0}{t}\ip{H(\theta_i-\theta^*),H(\theta_j-\theta^*)}=\E\ous{\sum}{i=0}{t}\ip{H(\theta_i-\theta^*),H(\theta_j-\theta^*)}+ 2\E\ous{\sum}{i=0}{t-1}\ous{\sum}{j=i+1}{t}\ip{H(\theta_i-\theta^*),H(\theta_j-\theta^*)}$. Now
\begin{align}\label{inter}
&\E\ous{\sum}{i=0}{t-1}\ous{\sum}{j=i+1}{t}\ip{H(\theta_i-\theta^*),H(\theta_j-\theta^*)}\nn\\
&=\E\ous{\sum}{i=0}{t-1}\ous{\sum}{j=i+1}{t}\ip{H(\theta_i-\theta^*),H\big[F_{j,i+1} (\theta_i-\theta^*)+\alpha\sum_{k=i+1}^j F_{j,k+1}\zeta_{k}\big]}\nn\\
&=\E\ous{\sum}{i=0}{t-1}\ous{\sum}{j=i+1}{t}\ip{H(\theta_i-\theta^*),H F_{j,i+1} (\theta_i-\theta^*)}\nn\\
&=\E\ous{\sum}{i=0}{t-1}\ous{\sum}{j=i+1}{t}\ip{H(\theta_i-\theta^*),H(I-\alpha H)^{j-i} (\theta_i-\theta^*)}\nn\\
&=2(\alpha\rho_H)^{-1}\E\ous{\sum}{i=0}{t-1}\ip{H(\theta_i-\theta^*),H (\theta_i-\theta^*)}\nn\\
&\leq2(\alpha\rho_H)^{-1}\E\ous{\sum}{i=0}{t}\ip{H(\theta_i-\theta^*),H (\theta_i-\theta^*)}\nn\\
\end{align}
$\E\ous{\sum}{i=0}{t}\ous{\sum}{j=0}{t}\ip{H(\theta_i-\theta^*),H(\theta_j-\theta^*)}=\E\ous{\sum}{i=0}{t}(1+4(\alpha\rho_H)^{-1})\ip{H(\theta_i-\theta^*),H(\theta_i-\theta^*)}$

Now
\begin{align*}
\E\ip{H(\theta_i-\theta^*),H(\theta_i-\theta^*)}=\E\ip{F_{i,1}e_0,F_{i,1}e_0}+\ous{\sum}{j=1}{i}\E\ip{F_{i,j+1}\zeta_j,F_{i,j+1}\zeta_j}
\leq (1-\alpha\rho_H)^i+ (\alpha\rho_H)^{-1}\sigma^2
\end{align*}
$\E\ous{\sum}{i=0}{t}\ous{\sum}{j=0}{t}\ip{H(\theta_i-\theta^*),H(\theta_j-\theta^*)}\leq (1+4(\alpha\rho_H)^{-1}) (\alpha\rho_H)^{-1}(t\sigma^2+\norm{\theta_0-\ts}^2)$
\begin{align}
\E[\norm{H\eb_t}]\leq \frac{1}{(t+1)^2}
\end{align}


\begin{align*}
\E<A(\theta_t-\theta^*),(\theta_t-\theta^*)>&=g^0_t(\theta_0-\theta^*)+\alpha\sum_{k=0}^t g^{k+1}_t(M_{k+1})\\
\sum_{i=0}^t\E<A(\theta_i-\theta^*),(\theta_i-\theta^*)>&=\sum_{i=0}^t g^0_i(\theta_0-\theta^*)+\alpha\sum_{k=0}^t g^{k+1}_i(M_{k+1})\\
&\leq\alpha^{-1}(f^0_0(\theta_0-\ts)-f^0_{t+1}(\theta_0-\ts))+\sum_{k=0}^t \alpha^{-1}(f^k_k(M_{k+1})-f^k_{t+1}(M_{k+1}))\\
&\leq\alpha^{-1}(f^0_0(\theta_0-\ts))+\alpha^{-1}(t+1)\sigma\sum_{k=0}^t \alpha^{-1}(f^k_k(M_{k+1}))\\
&\leq\alpha^{-1}\parallel \theta_0-\ts\parallel^2+\alpha^{-1}(t+1)\sigma^2
\end{align*}
\begin{lemma}
In \eqref{inter} $C_t\leq \frac{t+1}{\rho}{(1-\alpha\rho)^{t+1}}$
\end{lemma}
\begin{proof}
\begin{align*}
\E<A(\theta_i-\theta^*),(\theta_i-\theta^*)>&=g^0_i(\theta_0-\theta^*)+\alpha\sum_{k=0}^i g^{k+1}_i(M_{k+1})\\
\end{align*}
\end{proof}
\comment{
\begin{proof}
\begin{align*}
&<A(\theta_i-\theta^*),(I-\alpha A)^{t-i+1} (\theta_i-\theta^*)>\\
&\leq(1-\alpha \rho)^{t-i+1} <(\theta_t-\theta^*),A (\theta_t-\theta^*)>\\
\end{align*}
\begin{align*}
C_t&=\E\sum_{i=0}^t<A(\theta_i-\theta^*),(I-\alpha A)^{t-i+1} (\theta_i-\theta^*)>\\
&\leq\E\sum_{i=0}^t|<A(\theta_i-\theta^*),(I-\alpha A)^{t-i+1} (\theta_i-\theta^*)>|\\
&\leq \E\sum_{i=0}^t(1-\alpha\rho)^{t-i+1}(1-\alpha\rho)^i\\
&\leq \frac{t+1}{\rho}{(1-\alpha\rho)^{t+1}}\\
&\E<\theta_i-\theta^*,\theta_j-\theta^*>\\
&=\alpha^2\E\sum_{k=1}^i\sum_{j=1}^i <F_{i,j+1}M_{j+1},F_{i,k+1} M_{k+1}>\\
&=\alpha^2\E\sum_{k=1}^i<F_{i,k+1}M_{k+1},F_{i,k+1} M_{k+1}>\\
\end{align*}
\end{proof}
\begin{align*}
&\E[<F_{i,k+1}M_{k+1},F_{i,k+1} M_{k+1}>]\\
&=\E[\big[\Big[\bigg[<F_{i,k+1} M_{k+1},F_{i,k+1} M_{k+1}>|\F_{j-1}\bigg]|F_{j-2}\Big]\ldots|\F_{k+1}\big]]\\
&\leq(1-\alpha\rho)^{i-k-1}\sigma^2\\
&\E<\theta_i-\theta^*,\theta_j-\theta^*>\\
&\leq \frac{\alpha\sigma^2}{\rho}\\
&\E[<F_{i,1}(\theta_0-\theta^*),F_{i,1}(\theta_0-\theta^*)>]\\
&=\E[\bigg[\Big[\big[<F_{i,1}(\theta_0-\theta^*),F_{i,1}(\theta_0-\theta^*)>|\F_{j-1}\big]|F_{j-2}\Big]\ldots|\F_{k+1}\bigg]]\\
&\leq (1-\alpha\rho)^{i-k-1}\parallel \theta_0-\theta^*\parallel\\
&\leq (\rho\alpha)^{-1}\parallel \theta_0-\theta^*\parallel
\end{align*}
}
